Helpers for arrays of leaf_packages

fstar/new/TreeSync.Helpers.fst
@@ -19,6 +19,23 @@ let rec mk_path_aux (l:nat) (i:index_n l) (sonp:Seq.seq (option node_package_t){
 /// Helpers
 ///
 
+type leaf_array_t (sz:nat) = a:array (option leaf_package_t){length a = sz}
+
+(* Retreives the array of leaf_packages from the tree *)
+let rec tree_leaf_packages (l:nat) (t:tree_t l): leaf_array_t (pow2 l) =
+  match t with
+  | Leaf _ olp ->
+    (match olp with
+    | None -> singleton None
+    | Some lp -> singleton (Some lp))
+  | Node _ _ left right -> append (tree_leaf_packages (l-1) left)
+				 (tree_leaf_packages (l-1) right)
+
+(* Retreives the array of leaf_packages from the state *)
+val leaf_packages: st:state_t -> leaf_array_t (max_size st)
+let leaf_packages st = tree_leaf_packages st.st_levels st.st_tree
+
+
 (* Create a path for from a sequence of node packages *)
 val mk_path: l:nat -> Seq.seq (option node_package_t) -> option leaf_package_t
   -> Tot (option (path_t l))
@@ -26,4 +43,3 @@ val mk_path: l:nat -> Seq.seq (option node_package_t) -> option leaf_package_t
 let rec mk_path l sonp olp =
   if l = 0 || length sonp + 1 <> l then None
   else Some (mk_path_aux l 0 sonp olp)
-
